Separate computation from logic

Sort.v
@@ -1,46 +1,25 @@
 Load List.
 
-Class DecidableBinaryRelation {A} (r : A -> A -> Prop) := {
-  decide_binary_relation : A -> A -> bool;
-  DecidableBinaryRelation_spec : forall a b, reflect (r a b) (decide_binary_relation a b);
+Class DecidableBinaryRelation {A} (r : A -> A -> Prop) (rb : A -> A -> bool) := {
+  DecidableBinaryRelation_spec : forall a b, reflect (r a b) (rb a b);
 }.
 
-Arguments decide_binary_relation {A}%type_scope r%function_scope {DecidableBinaryRelation} _ _.
-Arguments DecidableBinaryRelation_spec {A}%type_scope r%function_scope {DecidableBinaryRelation} _ _.
+Arguments DecidableBinaryRelation_spec {A}%type_scope r%function_scope {rb}%function_scope
+  {DecidableBinaryRelation} _.
 
 Class TotalOrder {A} (r : A -> A -> Prop) := {
-  TotalOrder_DecidableBinaryRelation :> DecidableBinaryRelation r;
   TotalOrder_reflexivity : forall a, r a a;
   TotalOrder_transitivity : forall a b c, r a b -> r b c -> r a c;
   TotalOrder_antisymmetry : forall a b, r a b -> r b a -> a = b;
   TotalOrder_totality : forall a b, r a b \/ r b a;
 }.
 
-Coercion TotalOrder_DecidableBinaryRelation : TotalOrder >-> DecidableBinaryRelation.
 Arguments TotalOrder_reflexivity {A}%type_scope r%function_scope {TotalOrder} _.
 Arguments TotalOrder_transitivity {A}%type_scope r%function_scope {TotalOrder} _ _ _ _ _.
 Arguments TotalOrder_antisymmetry {A}%type_scope r%function_scope {TotalOrder} _ _ _ _.
 Arguments TotalOrder_totality {A}%type_scope r%function_scope {TotalOrder} _ _.
 
-Class CostTotalOrder {A} (r : A -> A -> Prop) := {
-  CostTotalOrder_TotalOrder :> TotalOrder r;
-  CostTotalOrder_cost : Cost (Signature [_; _] _) (decide_binary_relation r);
-}.
-
-Coercion CostTotalOrder_TotalOrder : CostTotalOrder >-> TotalOrder.
-Arguments CostTotalOrder_cost {A}%type_scope r%function_scope {CostTotalOrder}.
-
-Class CostConstantTotalOrder {A} (r : A -> A -> Prop) := {
-  CostConstantTotalOrder_CostTotalOrder :> CostTotalOrder r;
-  CostConstantTotalOrder_cost_constant : binary_cost_constant (CostTotalOrder_cost r);
-}.
-
-Coercion CostConstantTotalOrder_CostTotalOrder : CostConstantTotalOrder >-> CostTotalOrder.
-Arguments CostConstantTotalOrder_cost_constant {A}%type_scope r%function_scope {CostConstantTotalOrder}.
-
-#[export, program] Instance nat_le_DecidableBinaryRelation : DecidableBinaryRelation Nat.le := {
-  decide_binary_relation := Nat.leb;
-}.
+#[export, program] Instance nat_le_DecidableBinaryRelation : DecidableBinaryRelation Nat.le Nat.leb.
 Next Obligation.
   apply Nat.leb_spec0.
 Qed.
@@ -59,13 +38,6 @@ Qed.
 #[export, program] Instance nat_leb_Cost : Cost (Signature [_; _] _) Nat.leb := {
   cost_fun := fun _ _ => 1;
 }.
-
-#[export, program] Instance nat_le_CostTotalOrder : CostTotalOrder Nat.le.
-
-#[export, program] Instance nat_le_CostConstantTotalOrder : CostConstantTotalOrder Nat.le.
-Next Obligation.
-  exists 1. intros ?. simpl. destruct a. lia.
-Qed.
 
 Fixpoint sorted {A} r {total_order : TotalOrder r} (l : list A) :=
   match l with
@@ -103,16 +75,22 @@ Proof.
         -- apply IHl. simpl. auto.
 Qed.
 
-Definition locally_sortedb {A} r {total_order : TotalOrder r} :=
-  fix locally_sortedb (l : list A) :=
+Definition locally_sortedb_impl {A} rb :=
+  fix locally_sortedb_impl (l : list A) :=
     match l with
     | [] => true
     | [_] => true
-    | x :: ((y :: _) as l') => decide_binary_relation r x y && locally_sortedb l'
+    | x :: ((y :: _) as l') => rb x y && locally_sortedb_impl l'
     end.
 
+Definition locally_sortedb {A} (r : A -> A -> Prop) {total_order : TotalOrder r}
+  {rb} {decidable_binary_relation : DecidableBinaryRelation r rb} :=
+  locally_sortedb_impl rb.
+
 Theorem locally_sortedb_spec :
-  forall {A} r {total_order : TotalOrder r} (l : list A),
+  forall {A} r {total_order : TotalOrder r}
+    {rb} {decidable_binary_relation : DecidableBinaryRelation r rb}
+    (l : list A),
   reflect (locally_sorted r l) (locally_sortedb r l).
 Proof.
   intros ? ? ? ?. induction l.
@@ -123,32 +101,28 @@ Proof.
       destruct (DecidableBinaryRelation_spec r a b); destruct IHl; constructor; intuition auto.
 Qed.
 
-Definition locally_sortedb_cost {A} r {total_order : CostTotalOrder r} :=
+Definition locally_sortedb_impl_cost {A} rb {rb_Cost: Cost (Signature [_; _] _) rb} :=
   ltac2:(
     Cost.refine_compute_cost
-    [
-      (
-        ('(@decide_binary_relation _ _ total_order), 2),
-        '(@cost_fun _ _ (@CostTotalOrder_cost _ _ total_order))
-      )
-    ]
+    [(('rb, 2), '(@cost_fun _ _ rb_Cost))]
     1
-    (eval red in (@locally_sortedb A r total_order))
+    (eval red in (@locally_sortedb_impl A rb))
     []
   ).
 
-Theorem locally_sortedb_cost_linear_on_cost_constant_total_order :
-  forall {A} r {total_order : CostConstantTotalOrder r},
+Theorem locally_sortedb_impl_cost_linear_on_cost_constant_rb :
+  forall {A} r {total_order : TotalOrder r}
+    {rb} {decidable_binary_relation : DecidableBinaryRelation r rb} {rb_Cost: Cost (Signature [_; _] _) rb},
+  binary_cost_constant rb_Cost ->
   big_o
-    (locally_sortedb_cost r)
+    (locally_sortedb_impl_cost rb)
     (fun (l : list A) => 1 + length l).
 Proof.
-  intros ? ? ?. destruct total_order as (total_order & (c & H)). exists (c + 18). intros l. induction l.
+  intros ? ? ? ? ? ? ?. destruct H as (c & H). exists (c + 18). intros l. induction l.
   - simpl. lia.
   - simpl. destruct l.
     + lia.
-    + rename a0 into b. unfold CostConstantTotalOrder_CostTotalOrder in IHl.
-      specialize (H (a, b)). simpl in H. lia.
+    + rename a0 into b. specialize (H (a, b)). lia.
 Qed.
 
 Definition is_sorter {A} r {total_order : TotalOrder r} f :=
@@ -206,22 +180,28 @@ Proof.
     + apply is_permutation_sym. auto.
 Qed.
 
-Definition insert_sorted {A} r {total_order : TotalOrder r} :=
-  fix insert_sorted a (l : list A) :=
+Definition insert_sorted_impl {A} rb :=
+  fix insert_sorted_impl a (l : list A) :=
     match l with
     | [] => [a]
     | x :: l' =>
-      if decide_binary_relation r a x
+      if (rb a x : bool)
       then a :: x :: l'
-      else x :: (insert_sorted a l')
+      else x :: (insert_sorted_impl a l')
     end.
 
+Definition insert_sorted {A} (r : A -> A -> Prop) {total_order : TotalOrder r}
+  {rb} {decidable_binary_relation : DecidableBinaryRelation r rb} :=
+  insert_sorted_impl rb.
+
 Theorem insert_sorted_correct :
-  forall {A} r {total_order : TotalOrder r} a (l : list A),
+  forall {A} r {total_order : TotalOrder r}
+    {rb} {decidable_binary_relation : DecidableBinaryRelation r rb}
+    a (l : list A),
   sorted r l ->
   is_permutation (insert_sorted r a l) (a :: l) /\ sorted r (insert_sorted r a l).
 Proof.
-  intros ? ? ? ? ? ?. induction l.
+  intros ? ? ? ? ? ? ? ?. induction l.
   - simpl. split.
     + apply is_permutation_add. apply is_permutation_empty.
     + auto.
@@ -249,61 +229,67 @@ Proof.
         -- auto.
 Qed.
 
-Definition insert_sorted_cost {A} r {total_order : CostTotalOrder r} :=
+Definition insert_sorted_impl_cost {A} rb {rb_Cost: Cost (Signature [_; _] _) rb} :=
   ltac2:(
     Cost.refine_compute_cost
-    [
-      (
-        ('(@decide_binary_relation _ _ total_order), 2),
-        '(@cost_fun _ _ (@CostTotalOrder_cost _ _ total_order))
-      )
-    ]
+    [(('rb, 2), '(@cost_fun _ _ rb_Cost))]
     2
-    (eval red in (@insert_sorted A r total_order))
+    (eval red in (@insert_sorted_impl A rb))
     []
   ).
 
-Theorem insert_sorted_cost_linear_on_cost_constant_total_order :
-  forall {A} r {total_order : CostConstantTotalOrder r},
+Theorem insert_sorted_cost_linear_on_cost_constant_rb :
+  forall {A} r {total_order : TotalOrder r}
+    {rb} {decidable_binary_relation : DecidableBinaryRelation r rb}
+    {rb_Cost: Cost (Signature [_; _] _) rb},
+  binary_cost_constant rb_Cost ->
   big_o
-    (fun '(a, l) => insert_sorted_cost r a l)
+    (fun '(a, l) => insert_sorted_impl_cost rb a l)
     (fun '(_, l) => 1 + length (l : list A)).
 Proof.
-  intros ? ? ?. destruct total_order as (total_order & (c & H)). exists (c + 19). intros (a, l). induction l.
+  intros ? ? ? ? ? ? ?. destruct H as (c & H). exists (c + 19). intros (a, l). induction l.
   - simpl. lia.
-  - rename a0 into b. unfold CostConstantTotalOrder_CostTotalOrder in IHl. simpl. specialize (H (a, b)).
-    destruct (DecidableBinaryRelation_spec r a b); lia.
+  - rename a0 into b. simpl. specialize (H (a, b)). destruct (DecidableBinaryRelation_spec r a b); lia.
 Qed.
 
-Theorem insert_sorted_cost_constant_on_cost_constant_total_order_and_first_place :
-  forall {A} r {total_order : CostConstantTotalOrder r},
+Theorem insert_sorted_cost_constant_on_cost_constant_rb_and_first_place :
+  forall {A} r {total_order : TotalOrder r}
+    {rb} {decidable_binary_relation : DecidableBinaryRelation r rb}
+    {rb_Cost: Cost (Signature [_; _] _) rb},
+  binary_cost_constant rb_Cost ->
   constant
     (fun (p : {'(a, l) | list_forall (fun b => r a b) (l : list A)}) =>
       let 'exist _ (a, l) _ := p in
-        insert_sorted_cost r a l
+        insert_sorted_impl_cost rb a l
     ).
 Proof.
-  intros ? ? ?. destruct total_order as (total_order & (c & H0)). exists (c + 21). intros ((a, l), H). destruct l.
+  intros ? ? ? ? ? ? ?. destruct H as (c & H). exists (c + 21). intros ((a, l), H0). destruct l.
   - simpl. lia.
-  - rename a0 into b. simpl. specialize (H0 (a, b)). destruct (DecidableBinaryRelation_spec r a b).
+  - rename a0 into b. simpl. specialize (H (a, b)). destruct (DecidableBinaryRelation_spec r a b).
     + lia.
-    + simpl in H. intuition auto.
+    + simpl in H0. intuition auto.
 Qed.
 
-Definition insertion_sort {A} r {total_order : TotalOrder r} :=
-  fix insertion_sort (l : list A) :=
+Definition insertion_sort_impl {A} rb :=
+  fix insertion_sort_impl (l : list A) :=
     match l with
     | [] => []
-    | x :: l' => insert_sorted r x (insertion_sort l')
+    | x :: l' => insert_sorted_impl rb x (insertion_sort_impl l')
     end.
 
+Definition insertion_sort {A} (r : A -> A -> Prop) {total_order : TotalOrder r}
+  {rb} {decidable_binary_relation : DecidableBinaryRelation r rb} :=
+  insertion_sort_impl rb.
+
 Theorem insertion_sort_correct :
-  forall {A} (r : A -> A -> Prop) {total_order : TotalOrder r}, is_sorter r (insertion_sort r).
+  forall {A} (r : A -> A -> Prop) {total_order : TotalOrder r}
+    {rb} {decidable_binary_relation : DecidableBinaryRelation r rb},
+  is_sorter r (insertion_sort r).
 Proof.
-  unfold is_sorter. intros ? ? ? ?. induction l.
+  unfold is_sorter. intros ? ? ? ? ? ?. induction l.
   - simpl. auto using is_permutation_empty.
   - simpl. destruct IHl as (IHl1 & IHl2).
-    specialize (insert_sorted_correct r a (insertion_sort r l) IHl2) as (? & ?).
+    specialize (insert_sorted_correct _ a _ IHl2) as (? & ?).
     split.
     + apply is_permutation_trans with (a :: (insertion_sort r l)).
       * auto.
@@ -311,58 +297,62 @@ Proof.
     + auto.
 Qed.
 
-Definition insertion_sort_cost {A} r {total_order : CostTotalOrder r} :=
+Definition insertion_sort_impl_cost {A} rb {rb_Cost: Cost (Signature [_; _] _) rb} :=
   ltac2:(
     Cost.refine_compute_cost
-    [
-      (
-        ('(@insert_sorted A r total_order), 2),
-        '(@insert_sorted_cost A r total_order)
-      )
-    ]
+    [(('(@insert_sorted_impl A rb), 2), '(@insert_sorted_impl_cost _ rb rb_Cost))]
     1
-    (eval red in (@insertion_sort A r total_order))
-    ['(@insertion_sort A r total_order)]
+    (eval red in (@insertion_sort_impl A rb))
+    ['(@insertion_sort_impl A rb)]
   ).
 
-Theorem insertion_sort_cost_quadratic_on_cost_constant_total_order :
-  forall {A} r {total_order : CostConstantTotalOrder r},
+Theorem insertion_sort_cost_quadratic_on_cost_constant_rb :
+  forall {A} (r : A -> A -> Prop) {total_order : TotalOrder r}
+    {rb} {decidable_binary_relation : DecidableBinaryRelation r rb}
+    {rb_Cost: Cost (Signature [_; _] _) rb},
+  binary_cost_constant rb_Cost ->
   big_o
-    (insertion_sort_cost r)
+    (insertion_sort_impl_cost rb)
     (fun (l : list A) => 1 + (length l) * (length l)).
 Proof.
-  intros ? ? ?. destruct (insert_sorted_cost_linear_on_cost_constant_total_order r) as (c & H).
+  intros ? ? ? ? ? ? ?. destruct (insert_sorted_cost_linear_on_cost_constant_rb r H) as (c & H0).
   exists (c + 10). intros l. induction l.
   - simpl. lia.
   - simpl.
-    specialize (H (a, insertion_sort r l)). simpl in H.
-    replace (length (insertion_sort r l))
+    specialize (H0 (a, insertion_sort_impl rb l)). simpl in H0.
+    replace (length (insertion_sort_impl rb l))
       with (length l)
-      in H
-      by (apply permutation_length; apply insertion_sort_correct).
+      in H0
+      by (apply permutation_length; apply (insertion_sort_correct r)).
     lia.
 Qed.
 
 Theorem insertion_sort_cost_linear_on_cost_constant_total_order_and_list :
-  forall {A} r {total_order : CostConstantTotalOrder r},
+  forall {A} (r : A -> A -> Prop) {total_order : TotalOrder r}
+    {rb} {decidable_binary_relation : DecidableBinaryRelation r rb}
+    {rb_Cost: Cost (Signature [_; _] _) rb},
+  binary_cost_constant rb_Cost ->
   big_o
-    (fun (p : {l | sorted r l}) => let 'exist _ l _ := p in insertion_sort_cost r l)
+    (fun (p : {l | sorted r l}) => let 'exist _ l _ := p in insertion_sort_impl_cost rb l)
     (fun p => let 'exist _ l _ := p in 1 + length (l : list A)).
 Proof.
-  intros ? ? ?. destruct (insert_sorted_cost_constant_on_cost_constant_total_order_and_first_place r) as (c & H).
-  exists (c + 10). intros (l, H0). induction l.
+  intros ? ? ? ? ? ? ?.
+  destruct (insert_sorted_cost_constant_on_cost_constant_rb_and_first_place r H) as (c & H0).
+  exists (c + 10). intros (l, H1). induction l.
   - simpl. lia.
-  - simpl in H0. destruct H0 as (? & ?). apply IHl in H1. clear IHl. simpl.
-    apply list_forall_permutation with (l2 := insertion_sort r l) in H0.
-    + specialize (H ltac:(exists (a, (insertion_sort r l)); auto)). simpl in H. lia.
-    + apply is_permutation_sym. apply insertion_sort_correct.
+  - simpl in H1. destruct H1 as (? & ?). apply IHl in H2; clear IHl. simpl.
+    apply list_forall_permutation with (l2 := insertion_sort_impl rb l) in H1.
+    + specialize (H0 ltac:(exists (a, (insertion_sort_impl rb l)); auto)). simpl in H0. lia.
+    + apply is_permutation_sym. apply (insertion_sort_correct r).
 Qed.
 
 Section Example.
 
-Compute insertion_sort_cost _ [1; 1; 1; 1; 1; 1; 1; 1; 1; 1; 1; 1; 1; 1; 1; 1].
-Compute insertion_sort_cost _ [1; 2; 3; 4; 5; 6; 7; 8; 9; 10].
-Compute insertion_sort_cost _ [10; 9; 8; 7; 6; 5; 4; 3; 2; 1].
-Compute insertion_sort_cost _ [20; 19; 18; 17; 16; 15; 14; 13; 12; 11; 10; 9; 8; 7; 6; 5; 4; 3; 2; 1].
+Compute insertion_sort_impl_cost Nat.leb [1; 1; 1; 1; 1; 1; 1; 1; 1; 1; 1; 1; 1; 1; 1; 1].
+Compute insertion_sort_impl_cost Nat.leb [1; 2; 3; 4; 5; 6; 7; 8; 9; 10].
+Compute insertion_sort_impl_cost Nat.leb [10; 9; 8; 7; 6; 5; 4; 3; 2; 1].
+Compute insertion_sort_impl_cost Nat.leb [20; 19; 18; 17; 16; 15; 14; 13; 12; 11; 10; 9; 8; 7; 6; 5; 4; 3; 2; 1].
+
+Compute insertion_sort Nat.le [4; 4; 6; 1; 0; 40; 3].
 
 End Example.
